---
{"dg-publish":true,"permalink":"/linear-algebra/10-matrix-vector-multiplication/10-5-1-example-of-row-vector-matrix-multiplication-via-dot-products/","tags":["Type/Example","Topic/Linear_Algebra"]}
---

Types: *N/A*
Examples: *N/A*
Constructions: *N/A*
Generalizations: *N/A*

Properties: *N/A*
Sufficiencies: *N/A*
Questions: *N/A*

> [!example|*] Row-Vector-Matrix Multiplication via Dot Products
> Find the individual entries of $\vec{b} = \vec{x}^{T} \cdot A$ via [[Linear Algebra/10 Matrix-Vector Multiplication/10.5 Row-Vector-Matrix Multiplication via Dot Products\|10.5 Row-Vector-Matrix Multiplication via Dot Products]] where
> 
> $$
> \begin{align*}
> A = \begin{bmatrix}
> -3 & 4 & -3 \\
> -1 & 7 & 6 \\
> 0 & 1 & 2 \\
> 2 & -5 & -2
> \end{bmatrix} &&\text{and} && \vec{x}=\begin{bmatrix}
> 2 \\
> -1 \\
> 5 \\
> 3
> \end{bmatrix}
> \end{align*}
> $$

*Solution.* Recall our definition of row-vector-matrix multiplication via dot products.
$$
\begin{align*}
[\vec{b}]_{1\times n} &=  [\vec{x}^{T}]_{1 \times m} \cdot [A]_{m \times n}\\\\

\implies b_{k} &= \text{entry}_{(1,k)}(\vec{x}^{T} A)\\
&= \vec{x} \cdot A(:,k)\\
&= \sum_{i=1}^{m} a_{ik}x_{i}
\end{align*}
$$
Using our definition, let's first check if our inner dimensions agree.
$$
[\vec{b}]_{1 \times 3} = [\vec{x}^{T}]_{1 \times 4} \cdot [A]_{4 \times 3}
$$
- The inner dimensions agree.
- The outer dimensions provide our dimensions for output vector $\vec{b}$.

Now that we know the inner dimensions agree, we can generate our first output of $\vec{b}$.
$$
\begin{align*}
b_{1} &= \vec{x} \cdot A(:,1) &&\text{1. Dot product definition of RVMM}\\
&= \begin{bmatrix}
2 \\
-1 \\
5 \\
3
\end{bmatrix} \cdot \begin{bmatrix}
-3 \\
-1 \\
0 \\
2
\end{bmatrix}&&\text{2. Take inner product}\\
&= (2)(-3)+(-1)(-1)+(5)(0)+(3)(2)&&\text{3. Multiply out}\\
&= -6+1+0+6&&\text{4. Take sum of products}\\
&= 1&&\text{5. Final value of entry 1 of output vector}
\end{align*}
$$
We continue this process until $m=3$.
$$
\begin{align*}
\implies b_{2} &= \vec{x} \cdot A(:,2)\\
&= \begin{bmatrix}
2 \\
-1 \\
5 \\
3
\end{bmatrix} \cdot \begin{bmatrix}
4 \\
7 \\
1 \\
-5
\end{bmatrix}\\
&= (2)(4) + (-1)(7) + (5)(1)+(3)(-5)\\
&= 8 + -7 + 5 + -15\\
&= -9\\
\\
\implies b_{3} &= \vec{x} \cdot A(:,3)\\
&= \begin{bmatrix}
2 \\
-1 \\
5 \\
3
\end{bmatrix} \cdot \begin{bmatrix}
-3 \\
6 \\
2 \\
-2
\end{bmatrix}\\
&= (2)(-3)+(-1)(6)+(5)(2)+(3)(-2)\\
&= -6 + -6 + 10 + -6\\
&= -18
\end{align*}
$$
Finally, we can place each of our entry values into the appropriate column to form the vector
$$
\vec{b} = \begin{bmatrix}
b_{1} & b_{2} & b_{3}
\end{bmatrix} = \begin{bmatrix}
1 & -9 & -18
\end{bmatrix}
$$