---
{"dg-publish":true,"permalink":"/linear-algebra/11-matrix-matrix-multiplication/11-2-1-example-of-matrix-matrix-multiplication-via-linear-combination-of-columns/","tags":["Type/Example","Topic/Linear_Algebra"]}
---

Types: *N/A*
Examples: *N/A*
Constructions: *N/A*
Generalizations: *N/A*

Properties: *N/A*
Sufficiencies: *N/A*
Questions: *N/A*

> [!example] Matrix-Matrix Multiplication via Linear Combination of Columns
> 
> Let $A \in \mathbb{R}^{ 3 \times 2}$ and $X \in \mathbb{R}^{2 \times 3}$. Find the matrix-matrix product $B = A \cdot X$ using [[Linear Algebra/11 Matrix-Matrix Multiplication/11.2 Matrix-Matrix Multiplication via Linear Combination of Columns\|11.2 Matrix-Matrix Multiplication via Linear Combination of Columns]].
> $$
> A= \begin{bmatrix}
> 1 & 2 \\
> 3 & 4 \\
> 5 & 6
> \end{bmatrix}_{3 \times 2}, X = \begin{bmatrix}
> 1 & 2 & 3 \\
> 4 & 5 & 6
> \end{bmatrix}_{2 \times 3}
> $$


*Solution.* The inner dimensions are both equal to $2$, so we can do matrix-matrix multiplication. The outer dimensions are both $3$, so our output will be a $3 \times 3$ matrix. Through our linear combination of columns approach, we can find the resulting matrix through a column-by-column approach. 

Let's begin with column 1. Let's start by creating a general plan for what we are going to compute.
$$
\begin{align*}
B(:,1) &= A \cdot X(:,1)\\
&= \begin{bmatrix}
a_{11} & a_{12} \\
a_{21} & a_{22} \\
a_{31} & a_{32}
\end{bmatrix}_{2 \times 3} \cdot \begin{bmatrix}
x_{11} \\
x_{21}
\end{bmatrix}_{2 \times 1} &&\text{Matrix-vector product}\\
&= x_{11}\begin{bmatrix}
a_{11} \\
a_{21} \\
a_{31}
\end{bmatrix}+x_{21}\begin{bmatrix}
a_{12} \\
a_{22} \\
a_{32}
\end{bmatrix}&&\text{Linear combination}\\
&= \begin{bmatrix}
x_{11} \cdot a_{11} \\
x_{11}\cdot a_{21} \\
x_{11}\cdot a_{31}
\end{bmatrix} + \begin{bmatrix}
x_{21} \cdot a_{12} \\
x_{21} \cdot a_{22} \\
x_{21}  \cdot a_{32}
\end{bmatrix} && \text{Scalar-vector multiplication}\\
\implies B(:,1) &= \begin{bmatrix}
x_{11}a_{11}+x_{21}a_{12} \\
x_{11}a_{21}+x_{21}a_{22} \\
x_{11}a_{31}+x_{21}a_{32}
\end{bmatrix} && \text{Vector-vector addition}
\end{align*}
$$
Now that we have this in mind, let's plug in our values.
$$
\begin{align*}
\implies B(:,1) &= A \cdot X(:,1)\\
&= \begin{bmatrix}
1 & 2 \\
3 & 4 \\
5 & 6
\end{bmatrix}_{3 \times 2} \cdot \begin{bmatrix}
1 \\
4
\end{bmatrix}_{2 \times 1}\\
&= 1\begin{bmatrix}
1 \\
3 \\
5
\end{bmatrix}_{3 \times 1} + 4\begin{bmatrix}
2 \\
4 \\
6
\end{bmatrix}_{3 \times 1}\\
&= \begin{bmatrix}
1 \\
3 \\
5
\end{bmatrix}_{3 \times 1} + \begin{bmatrix}
8 \\
16 \\
24
\end{bmatrix}_{3 \times 1}\\
B(:,1)&= \begin{bmatrix}
9 \\
19 \\
29
\end{bmatrix}_{3 \times 1}
\end{align*}
$$
We continue this process for our column 2
$$
\begin{align*}
\implies B(:,2) &= A \cdot X(:,2)\\
&= \begin{bmatrix}
1 & 2 \\
3 & 4 \\
5 & 6
\end{bmatrix}_{3 \times 2} \cdot \begin{bmatrix}
2 \\
5
\end{bmatrix}_{2 \times 1}\\
&= 2 \begin{bmatrix}
1 \\
3 \\
5
\end{bmatrix}_{3 \times 1} + 5 \begin{bmatrix}
2 \\
4 \\
6
\end{bmatrix}_{3 \times 1}\\
&= \begin{bmatrix}
2 \\
6 \\
10
\end{bmatrix}_{3 \times 1} + \begin{bmatrix}
10 \\
20 \\
30
\end{bmatrix}_{3 \times 1}\\
B(:, 2) &= \begin{bmatrix}
12 \\
26 \\
40
\end{bmatrix}_{3 \times 1}
\end{align*}
$$
and column 3
$$
\begin{align*}
\implies B(:,3) &= A \cdot X(:, 3)\\
&= \begin{bmatrix}
1 & 2 \\
3 & 4 \\
5 & 6
\end{bmatrix}_{3 \times 2} \cdot \begin{bmatrix}
3 \\
6
\end{bmatrix}_{2 \times 1}\\
&= 3 \begin{bmatrix}
1 \\
3 \\
5
\end{bmatrix}_{3 \times 1} + 6 \begin{bmatrix}
2 \\
4 \\
6
\end{bmatrix}_{3 \times 1}\\
&= \begin{bmatrix}
3 \\
9 \\
15
\end{bmatrix}_{3 \times 1} + \begin{bmatrix}
12 \\
24 \\
36
\end{bmatrix}_{3 \times 1}\\
B(:,3) &= \begin{bmatrix}
15 \\
33 \\
51
\end{bmatrix}_{3 \times 1}
\end{align*}
$$
Putting our columns 1, 2, and 3 together, we get our final matrix-matrix product
$$
\begin{align*}
B &= A \cdot X\\
&= \begin{bmatrix}
1 & 2 \\
3 & 4 \\
5 & 6
\end{bmatrix}_{3 \times 2}\begin{bmatrix}
1 & 2 & 3 \\
4 & 5 & 6
\end{bmatrix}_{2 \times 2}\\
\implies B &= \begin{bmatrix}
9 & 12 & 15 \\
19 & 26 & 33 \\
29 & 40 & 51
\end{bmatrix}_{3 \times 3}
\end{align*}
$$

---

**Remark.** We can check our answer using [Octave](https://octave-online.net) with the following code:
```matlab
A = [1, 2; 3, 4; 5, 6]
X = [1, 2, 3; 4, 5, 6]
B = A * X
```
 <span style='float:right;'>$\blacklozenge$</span>

---

> [!example] Modify a single column of a matrix
> 
> Let a $4 \times 3$ modeling matrix $A$ be 
> $$
> [A]_{m \times n} = \begin{bmatrix}
> 1 & 0 & 0 \\
> -1 & 1 & 0 \\
> 0 & -1 & 1 \\
> 0 & 0 & -1
> \end{bmatrix}_{4 \times 3}
> $$
> Suppose we wish to double column 1 of $A$ and leave the other columns untouched. In other words, we want to multiply $A(:,1)$ by 2 and leave the other columns untouched.

*Solution.* Recall [[Linear Algebra/11 Matrix-Matrix Multiplication/11.1 Anatomy of Matrix-Matrix Multiplication\|11.1 Anatomy of Matrix-Matrix Multiplication]]. To do algebraic work on the columns of our modeling matrix, we can multiply on the right.

> [!question] What type of matrix would allow us to leave all other columns untouched?
> To double column 1 and leave all other columns untouched, we multiply on the right by a [[Linear Algebra/09 Matrix Arithmetic/9.9 Dilation Matrix\|9.9 Dilation Matrix]]. 
> 
<div class="transclusion internal-embed is-loaded"><a class="markdown-embed-link" href="/linear-algebra/09-matrix-arithmetic/9-9-dilation-matrix/#6d42e1" aria-label="Open link"><svg xmlns="http://www.w3.org/2000/svg" width="24" height="24" viewBox="0 0 24 24" fill="none" stroke="currentColor" stroke-width="2" stroke-linecap="round" stroke-linejoin="round" class="svg-icon lucide-link"><path d="M10 13a5 5 0 0 0 7.54.54l3-3a5 5 0 0 0-7.07-7.07l-1.72 1.71"></path><path d="M14 11a5 5 0 0 0-7.54-.54l-3 3a5 5 0 0 0 7.07 7.07l1.71-1.71"></path></svg></a><div class="markdown-embed">



> [!definition|*] Dilation Matrix
> 
> Let natural number $n \in \mathbb{N}$ and scalar $c \in \mathbb{R}$. For $j \in \{ 1,2,\dots,n \}$, we define an $n \times n$ **dilation matrix** 
> $
> D_{j}(c) = I_{n} + (c-1) \cdot \vec{e}_{j} \cdot \vec{e}_{j}^{T}
> $

</div></div>
 
> - Recall that a dilation matrix modifies the $j$th value of the [[Linear Algebra/08 Anatomy of Matrices/8.6 Identity Matrix\|8.6 Identity Matrix]]. 
> 
> Since we are trying to double column 1 of our modeling matrix $A$, we set $j=1$ and $c=2$ for our dilation matrix.


This is how our current setup would be written:
$$
\underset{ \text{modeling matrix} }{ [A]_{4 \times 3} } \cdot \underset{ \text{algebraic worker} }{ [D_{1}(2)]_{3 \times 3} } = \begin{bmatrix}
1 & 0 & 0 \\
-1 & 1 & 0 \\
0 & -1 & 1 \\
0 & 0 & -1
\end{bmatrix}_{4 \times 3}\begin{bmatrix}
2 & 0 & 0 \\
0 & 1 & 0 \\
0 & 0 & 1
\end{bmatrix}_{3 \times 3} = [B]_{4 \times 3}
$$
- We use an $n=3$ dilation matrix because we want the output matrix to have to same dimensions as the input (recall that the outer dimensions define the dimensions of $B$)

Let's compute our matrix-matrix product column-by-column.
$$
\begin{align*}
[B(:,1)] _{4 \times 1}&= \text{Column}_{1} (A \cdot D_{1}(2))\\
&= [A]_{4 \times 3} \cdot [\text{Column}_{1}(D_{1}(2))]_{3 \times 1}\\
&= \begin{bmatrix}
1 & 0 & 0 \\
-1 & 1 & 0 \\
0 & -1 & 1 \\
0 & 0 & -1
\end{bmatrix}_{4 \times 3} \cdot \begin{bmatrix}
2 \\
0 \\
0
\end{bmatrix}_{3 \times 1}\\
&= 2\begin{bmatrix}
1 \\
-1 \\
0 \\
0
\end{bmatrix}+0\begin{bmatrix}
0 \\
1 \\
-1 \\
0
\end{bmatrix}+0\begin{bmatrix}
0 \\
0 \\
1 \\
-1
\end{bmatrix}\\
&= \begin{bmatrix}
2 \\
-2 \\
0 \\
0
\end{bmatrix}+\begin{bmatrix}
0 \\
0 \\
0 \\
0
\end{bmatrix}+\begin{bmatrix}
0 \\
0 \\
0 \\
0
\end{bmatrix}\\
\implies [B(:,1)]_{4 \times 1} &= \begin{bmatrix}
2 \\
-2 \\
0 \\
0
\end{bmatrix}
\end{align*}
$$
Let's continue with column 2.
$$
\begin{align*}
[B(:,2)]_{4 \times 1} &=  \text{Column}_{2}(A \cdot D_{1}(2))\\
&= [A]_{4 \times 3} \cdot [\text{Column}_{2}(D_{1}(2))]_{3 \times 1}\\
&= \begin{bmatrix}
1 & 0 & 0 \\
-1 & 1 & 0 \\
0 & -1 & 1 \\
0 & 0 & -1
\end{bmatrix}_{4 \times 3} \cdot \begin{bmatrix}
0 \\
1 \\
0
\end{bmatrix}_{3 \times 1}\\
&= 0 \begin{bmatrix}
1 \\
-1 \\
0 \\
0
\end{bmatrix} + 1 \begin{bmatrix}
0 \\
1 \\
-1 \\
0
\end{bmatrix} + 0 \begin{bmatrix}
0 \\
0 \\
1 \\
-1
\end{bmatrix}\\
\implies [B(:,2)]_{4 \times 1} &= \begin{bmatrix}
0 \\
1 \\
-1 \\
0
\end{bmatrix}
\end{align*}
$$
Again, we continue with column 3.
$$
\begin{align*}
[B(:,3)]_{4 \times 1} &= \text{Column}_{3} (A \cdot D_{1}(2))\\
&= [A]_{4 \times 3} \cdot [\text{Column}_{3}(D_{1}(2))]\\
&= \begin{bmatrix}
1 & 0 & 0 \\
-1 & 1 & 0 \\
0 & -1 & 1 \\
0 & 0 & -1
\end{bmatrix}_{4 \times 3} \cdot \begin{bmatrix}
0 \\
0 \\
1
\end{bmatrix}_{3 \times 1}\\
&= 0 \begin{bmatrix}
1 \\
-1 \\
0 \\
0
\end{bmatrix}+0\begin{bmatrix}
0 \\
1 \\
-1 \\
0
\end{bmatrix}+1 \begin{bmatrix}
0 \\
0 \\
1 \\
-1
\end{bmatrix}\\
\implies [B(:,3)]_{4 \times 1} &= \begin{bmatrix}
0 \\
0 \\
1 \\
-1
\end{bmatrix}
\end{align*}
$$
Finally, we can combine our results to form our output.
$$
\begin{align*}
[A]_{4 \times 5} \cdot [D_{1}(2)] &= [B]_{4 \times 3}\\
\begin{bmatrix}
1 & 0 & 0 \\
-1 & 1 & 0 \\
0 & -1 & 0 \\
0 & 0 & -1
\end{bmatrix}_{4 \times 3} \begin{bmatrix}
2 & 0 & 0 \\
0 & 1 & 0 \\
0 & 0 & 1
\end{bmatrix}_{3 \times 3} &= \begin{bmatrix}
2 & 0 & 0 \\
-2 & 1 & 0 \\
0 & -1 & 0 \\
0 & 0 & -1
\end{bmatrix}_{4 \times 3}
\end{align*}
$$
Based on this example, we can generalize a pattern for scaling the $k$th column of matrix $A \in \mathbb{R}^{m \times n}$ by the number $c$. To scale the $k$th column of $A$, we multiply $A$ on the right by the $n \times n$ dilation matrix $D_{k}(c)$.


