---
{"dg-publish":true,"permalink":"/linear-algebra/11-matrix-matrix-multiplication/11-4-1-example-of-matrix-matrix-multiplication-via-dot-products/","tags":["Type/Example","Topic/Linear_Algebra"]}
---

Types: *N/A*
Examples: *N/A*
Constructions: *N/A*
Generalizations: *N/A*

Properties: *N/A*
Sufficiencies: *N/A*
Questions: *N/A*

> [!example|*] Matrix-Matrix Multiplication via Dot Products
> 
> Recall [[Linear Algebra/09 Matrix Arithmetic/9.8 Shear Matrix\|9.8 Shear Matrix]]. Let
> $$
> X=S_{21}(-3)=\begin{bmatrix}
> 1 & 0 \\
> -3 & 1
> \end{bmatrix} \text{ and } A = \begin{bmatrix}
> 2 & 1 & 2 \\
> 6 & 2 & 4
> \end{bmatrix}
> $$
> Use [[Linear Algebra/11 Matrix-Matrix Multiplication/11.4 Matrix-Matrix Multiplication via Dot Products\|11.4 Matrix-Matrix Multiplication via Dot Products]] to find entries of output
> $$
> B=XA
> $$

`\begin{proof}[Solution.]`
Since we are doing matrix-matrix multiplication via dot products, we will be finding $B$ using an entry-by-entry approach.
$$
B = \begin{bmatrix}
b_{11} & b_{12} & b_{13} \\
b_{21} & b_{22} & b_{23}
\end{bmatrix}_{2 \times 3}
$$
Let's compute the individual entries of $B$.
$$
\begin{align*}
b_{11} &= X(1,:)\cdot A(:,1)=\begin{bmatrix}
1 & 0
\end{bmatrix}\begin{bmatrix}
2 \\
6
\end{bmatrix}=1(2)+0(6)=2,\\
\\
b_{12}&= X(1,:)\cdot A(:,2)=\begin{bmatrix}
1 & 0
\end{bmatrix}\begin{bmatrix}
1 \\
2
\end{bmatrix}=1(1)+0(2)=1,\\
\\
b_{13}&= X(1,:)\cdot A(:,3)=\begin{bmatrix}
1 & 0
\end{bmatrix}\begin{bmatrix}
2 \\
4
\end{bmatrix}1(2)+0(4)=2,\\
\\
b_{21}&= X(2,:)\cdot A(:,1)=\begin{bmatrix}
-3 & 1
\end{bmatrix}\begin{bmatrix}
2 \\
6
\end{bmatrix}=-3(2)+1(6)=0,\\
\\
b_{22}&= X(2,:)\cdot A(:,2)=\begin{bmatrix}
-3 & 1
\end{bmatrix}\begin{bmatrix}
1 \\
2
\end{bmatrix}=-3(1)+1(2)=-1,\\
\\
b_{23}&= X(2,:) \cdot A(:,3)=\begin{bmatrix}
-3 & 1
\end{bmatrix}\begin{bmatrix}
2 \\
4
\end{bmatrix}=-3(2)+1(4)=-2
\end{align*}
$$
Putting this all together, we get
$$
\implies \begin{bmatrix}
1 & 0 \\
-3 & 1
\end{bmatrix}\begin{bmatrix}
2 & 1 & 2 \\
6 & 2 & 4
\end{bmatrix}= \begin{bmatrix}
2 & 1 & 2 \\
0 & -1 & 2
\end{bmatrix}
$$
`\end{proof}`