---
{"dg-publish":true,"permalink":"/linear-algebra/11-matrix-matrix-multiplication/11-7-applications-for-mass-spring-chain/","tags":["Type/Example","Topic/Linear_Algebra"]}
---

Types: *N/A*
Examples: *N/A*
Constructions: *N/A*
Generalizations: *N/A*

Properties: *N/A*
Sufficiencies: *N/A*
Questions: *N/A*

Recall [[Linear Algebra/03 Vector Modeling/3.1.2 Vector Model of Mass-Spring Chain\|3.1.2 Vector Model of Mass-Spring Chain]]. 

<div class="transclusion internal-embed is-loaded"><div class="markdown-embed">

<div class="markdown-embed-title">

# 600

</div>



==⚠  Switch to EXCALIDRAW VIEW in the MORE OPTIONS menu of this document. ⚠== You can decompress Drawing data with the command palette: 'Decompress current Excalidraw file'. For more info check in plugin settings under 'Saving'


# Excalidraw Data
## Text Elements
Spring Mass Chain at equilibrium
with NO external force (t=0 sec) 
Position
WITH external force 
-
x
+ 
-
u
+ 
## Embedded Files
3b1137dc3488130f0426281066cc4cdb86150ca1: $x_{1}$
28393dfb5fbbb11062a64a5349b3d2ad74216c6b: $x_{1}(t)$
b4c673079ee8391431f52a861441e23c282935ea: $x_{2}$
30ce668f797c9c1a4864fecddd89d649f36e9bbe: $x_{2}(t)$
b37230525c3687593a13ef4286596359b835cb6a: $m_1$
4220b76d93da23ed409042a358e0ba65cb445c12: $m_1$
67adcbf0e450fd865247abdf223b5fdbbfb6b193: $m_2$
bd3e400664b2f1c56c5dd7b6a03ec869ffd8a086: $m_2$
dbbee70a8808cc8d9dafe49327e52eaacb658d63: $u_{1}(t)$
49e1fa22f8b8a6dd52e6b8fa147915a9b6ce3144: $u_{2}(t)$



</div></div>

> [!exercise] Elongation Vector
> Let's derive a vector to represent the "stretch" of the springs.

`\begin{proof}[Solution.]`
To start, let's look at spring 1.

<div class="transclusion internal-embed is-loaded"><div class="markdown-embed">




==⚠  Switch to EXCALIDRAW VIEW in the MORE OPTIONS menu of this document. ⚠== You can decompress Drawing data with the command palette: 'Decompress current Excalidraw file'. For more info check in plugin settings under 'Saving'


# Excalidraw Data
## Text Elements
t = t (gravity on) 
t = 0 (gravity off) 
## Embedded Files
3b1137dc3488130f0426281066cc4cdb86150ca1: $x_{1}$
b37230525c3687593a13ef4286596359b835cb6a: $m_1$
dbbee70a8808cc8d9dafe49327e52eaacb658d63: $u_{1}(t)$
6882325161623e338accb43c8771cfdaa4197faa: $x(t)$
df1b694f998e3364fbab5f70737946345ad50344: $m_1$



</div></div>

$e_{1}(t)$ is the amount of "net" stretch of spring 1. Therefore,
$$
e_{1}(t) = u_{1}(t),
$$
which is the displacement value of mass 1.
- & Recall that [[Displacement\|displacement]] is the total change in position from the origin. 

Now, let's look at spring 2.

<div class="transclusion internal-embed is-loaded"><div class="markdown-embed">




==⚠  Switch to EXCALIDRAW VIEW in the MORE OPTIONS menu of this document. ⚠== You can decompress Drawing data with the command palette: 'Decompress current Excalidraw file'. For more info check in plugin settings under 'Saving'


# Excalidraw Data
## Text Elements
t = 0 (gravity off) 
t = t (gravity on) 
## Embedded Files
3b1137dc3488130f0426281066cc4cdb86150ca1: $x_{1}$
b37230525c3687593a13ef4286596359b835cb6a: $m_1$
dbbee70a8808cc8d9dafe49327e52eaacb658d63: $u_{1}(t)$
2b9c56ed80c981bbb5f02641ced8a7fd94707db3: $m_2$
0f8efe5da3d0ccba263eb2de81dfb683ecd6af85: $k_1$
9b86fb105f7d44ddc4b5888c3752f57945da3c2e: $m_1$
430b663027aa368f769331fc130fb7014daa86c1: $m_2$
29277912adeba9fccf8152bc585678d9cfd6401c: $k_2$
a874b27e0dbc1176a3998bb4d600f1192bb4b9a1: $x_{2}$
d7467b0de22780e942654b10d61bd6a220af74f4: $u_{2}(t)$



</div></div>

Suppose $m_{1}$ had 0 displacement.
$$
\implies u_{1}(t) = 0
$$
How much would $m_{2}$ drop?
$$
\begin{align*}
e_{2}(t) &= \text{amount of "net" stretch of spring 2 at time }t\\
&= u_{2}(t)-u_{1}(t)
\end{align*}
$$

---

**Remark.** Hooke's law is more about ==elongation== than displacement. This is because we are assuming the frame of reference is at a fixed point ($m_{1}$ does not move). In other words, the possible movement of the top spring is not factored in.
 <span style='float:right;'>$\blacklozenge$</span>

---

Lastly, let's look at the bottom spring, spring 3.

<div class="transclusion internal-embed is-loaded"><div class="markdown-embed">




==⚠  Switch to EXCALIDRAW VIEW in the MORE OPTIONS menu of this document. ⚠== You can decompress Drawing data with the command palette: 'Decompress current Excalidraw file'. For more info check in plugin settings under 'Saving'


# Excalidraw Data
## Text Elements
t = 0 (gravity off) 
t = t (gravity on) 
## Embedded Files
3b1137dc3488130f0426281066cc4cdb86150ca1: $x_{2}$
2b9c56ed80c981bbb5f02641ced8a7fd94707db3: $m_2$
430b663027aa368f769331fc130fb7014daa86c1: $m_2$
29277912adeba9fccf8152bc585678d9cfd6401c: $k_2$
a874b27e0dbc1176a3998bb4d600f1192bb4b9a1: $x_{1}$
d7467b0de22780e942654b10d61bd6a220af74f4: $u_{2}(t)$
24ced6f765d89376cd660f19a00cf869b9092901: $k_2$



</div></div>

$$
\begin{align*}
e_{3}(t) &= \text{elongation of spring 3 at time }t\\
&= \underbrace{ -u_{2}(t) }_{ \text{negative of displacement} }
\end{align*}
$$
- When elongation is negative, the spring length is shorter than it's original length.

---

**Remark.** When $u_{2}$ is positive, the spring is stretched and vice versa.
 <span style='float:right;'>$\blacklozenge$</span>

---

Now that we have our elongation values, we can create our elongation vector
$$
\vec{e}(t) = \begin{bmatrix}
e_{1}(t) \\
e_{2}(t) \\
e_{3}(t)
\end{bmatrix}= \begin{bmatrix}
u_{1}(t) \\
u_{2}(t)-u_{1}(t)  \\
-u_{2}(t)
\end{bmatrix}
$$
Can we rewrite this as a [[Linear Algebra/06 Span and Linear Independence/6.1 Linear Combination of Vectors\|6.1 Linear Combination of Vectors]]?
$$
\begin{align*}
&= \begin{bmatrix}
u_{1}(t)+0 \\
u_{2}(t)-u_{1}(t) \\
0-u_{2}(t)
\end{bmatrix}\\
&= \begin{bmatrix}
u_{1}(t) \\
-u_{1}(t) \\
0
\end{bmatrix} + \begin{bmatrix}
0 \\
u_{2}(t) \\
-u_{2}(t)
\end{bmatrix}\\
\implies \vec{e}(t) &= \underbrace{ u_{1}(t)\begin{bmatrix}
1 \\
-1 \\
0
\end{bmatrix} }_{ \text{scalar} \times \text{column vector} }+\underbrace{ u_{2}(t)\begin{bmatrix}
0 \\
1 \\
-1
\end{bmatrix} }_{ \text{scalar} \times \text{column vector} }
\end{align*}
$$
Recall the definition of [[Linear Algebra/10 Matrix-Vector Multiplication/10.1 Matrix-Column-Vector Multiplication via Linear Combinations\|10.1 Matrix-Column-Vector Multiplication via Linear Combinations]]. We can rewrite our elongation vector as a matrix vector multiplication problem.
$$
\begin{align*}
&= \begin{bmatrix}
1 & 0 \\
-1 & 1 \\
0 & -1
\end{bmatrix}_{3 \times 2}\begin{bmatrix}
u_{1}(t) \\
u_{2}(t)
\end{bmatrix}_{2 \times 1} \\
&= \underset{ \text{modeling matrix} }{ A } \cdot \underset{ \text{algebraic worker} }{ \vec{u}(t) }
\end{align*}
$$
Recall when the algebraic worker is on the right and the modeling matrix is on the left, we work with columns.
`\end{proof}`

---

> [!exercise] Net Spring Force Vector
> Now that we have our elongation matrix, we can come up with our force vector.

`\begin{proof}[Solution.]`
Let $f_{si}(t)$ be the net change in stored force of spring $i$. Then, our force vector
$$
\begin{align*}
\vec{f}_{s} &= \begin{bmatrix}
f_{s_{1}}(t) \\
f_{s_{2}}(t) \\
f_{s_{3}}(t)
\end{bmatrix}\\
&= \begin{bmatrix}
k_{1} \cdot e_{1}(t) \\
k_{2} \cdot e_{2}(t) \\
k_{3} \cdot e_{3}(t)
\end{bmatrix}
\end{align*}
$$

 ---
 **Remark.** At rest, the springs are at a nonzero force. They are still able to do work. If you were to cut one of the springs, it would snap away. However, we can use this force value as our ==reference point for net zero==.

 <span style='float:right;'>$\blacklozenge$</span>

---

Can we rewrite our force vector as a linear combination?
$$
\begin{align*}
&= \begin{bmatrix}
k_{1}e_{1}(t)+0+0 \\
0+k_{2}e_{2}(t)+0 \\
0+0+k_{3}e_{3}(t)
\end{bmatrix}\\
&= \begin{bmatrix}
k_{1}e_{1}(t) \\
0 \\
0
\end{bmatrix}+ \begin{bmatrix}
0 \\
k_{2}e_{2}(t) \\
0
\end{bmatrix}+\begin{bmatrix}
0 \\
0 \\
k_{3}e_{3}(t)
\end{bmatrix}
\end{align*}
$$
In this case, we think of the scalars as the function $e(t)$.
$$
\begin{align*}
&= e_{1}(t)\begin{bmatrix}
k_{1} \\
0 \\
0
\end{bmatrix} + e_{2}(t) \begin{bmatrix}
0 \\
k_{2} \\
0
\end{bmatrix} + e_{3}(t) \begin{bmatrix}
0 \\
0 \\
k_{3}
\end{bmatrix}\\
&= \underbrace{ \begin{bmatrix}
k_{1} & 0 & 0 \\
0 & k_{2} & 0 \\
0 & 0 & k_{3}
\end{bmatrix}_{3 \times 3} }_{ \text{diagonal matrix!} } \begin{bmatrix}
e_{1}(t) \\
e_{2}(t) \\
e_{3}(t)
\end{bmatrix}_{3 \times 1}\\
\implies \vec{f}_{s} &= \mathbb{C} \cdot \vec{e}(t)
\end{align*}
$$
Note that we don't use $K$ because that's reserved for other types of really important problems in fields like engineering.
- [ ] Why do we think of the scalars as $e(t)$? #question
`\end{proof}`

---

> [!exercise] Net Force Equation
> Let's find the net force $\sum F$ on each mass.

`\begin{proof}[Solution.]`
$$
\begin{align*}
\sum F &= m \cdot a\\
\implies \sum F &= m \cdot \ddot{u}
\end{align*}
$$

$$
\begin{align*}
\underbrace{ \vec{e}(t) }_{ \text{elongation vector} } &= A d(t)\\
\implies \vec{f}_{s}(t) &= \mathbb{C} \vec{e}(t)
\end{align*}
$$

Let's look at a free body diagram of mass 1.

<div class="transclusion internal-embed is-loaded"><div class="markdown-embed">




==⚠  Switch to EXCALIDRAW VIEW in the MORE OPTIONS menu of this document. ⚠== You can decompress Drawing data with the command palette: 'Decompress current Excalidraw file'. For more info check in plugin settings under 'Saving'


# Excalidraw Data
## Text Elements
## Embedded Files
c2795b29c6b4b41c00e7efb24af126f874d69867: $m_1$
df96b708c1e5a71cdfcd8a0ec614029ea8c170ca: $f_{e_{1}}$
ae018fe332f098ed770d390dabe4faae8d71f9b8: $f_{s_{2}}$
30a6d1cf6c17361a7bb5f29dcdc195f7d8637d3a: $f_{s_{1}}$



</div></div>


$$
\begin{align*}
y_{1}(t) &= \text{net internal force on } m_{1}\\
&= -f_{s_{1}}(t) + f_{s_{2}}(t) + f_{e_{1}}(t)
\end{align*}
$$
- $f_{e_{1}}(t)$ is the external force applied to $m_{1}$ (ex. gravity, shaking, etc.)

Let's look at the free body diagram mass 2.

<div class="transclusion internal-embed is-loaded"><div class="markdown-embed">




==⚠  Switch to EXCALIDRAW VIEW in the MORE OPTIONS menu of this document. ⚠== You can decompress Drawing data with the command palette: 'Decompress current Excalidraw file'. For more info check in plugin settings under 'Saving'


# Excalidraw Data
## Text Elements
## Embedded Files
c2795b29c6b4b41c00e7efb24af126f874d69867: $m_1$
df96b708c1e5a71cdfcd8a0ec614029ea8c170ca: $f_{e_{2}} (t)$
ae018fe332f098ed770d390dabe4faae8d71f9b8: $f_{s_{3}} (t)$
30a6d1cf6c17361a7bb5f29dcdc195f7d8637d3a: $f_{s_{2}} (t)$



</div></div>

$$
\begin{align*}
y_{2}(t) &= \text{net focus on } m_{2}\\
&= -f_{s_{2}}(t) + f_{s_{3}}(t) + f_{e_{2}}(t)
\end{align*}
$$
Therefore, our net force equation is
$$
\begin{align*}
\underset{ \text{net forces on masses} }{ \left[ \sum \vec{F}(t) \right]_{2 \times 1} } &= \begin{bmatrix}
\sum F_{1}(t) \\
\sum F_{2}(t)
\end{bmatrix}\\
&= \begin{bmatrix}
-f_{s_{1}}(t) + f_{s_{2}}(t) + f_{e_{1}}(t) \\
-f_{s_{2}}(t) + f_{s_{3}}(t) + f_{e_{2}}(t)
\end{bmatrix}
\end{align*}
$$
- & Note that the $\sum$ sign is used as the name of the vector.

We can break this vector into two pieces.
$$
= \underbrace{ \begin{bmatrix}
-f_{s_{1}}(t)+f_{s_{2}}(t) \\
-f_{s_{2}}(t) + f_{s_{3}}(t)
\end{bmatrix} }_{ \text{internal forcces} } + \underbrace{ \begin{bmatrix}
f_{e_{1}}(t) \\
f_{e_{2}}(t)
\end{bmatrix} }_{ \text{external forces} }
$$
What would happen if we factored out the negative?
$$
= - \begin{bmatrix}
f_{s_{1}}(t)-f_{s_{2}}(t)+0 \\
0+f_{s_{2}}(t)-f_{s_{3}}(t)
\end{bmatrix} + \begin{bmatrix}
f_{e_{1}}(t) \\
f_{e_{2}}(t)
\end{bmatrix}
$$
Do you see a [[Linear Algebra/06 Span and Linear Independence/6.1 Linear Combination of Vectors\|6.1 Linear Combination of Vectors]]?
$$
= -\left( \begin{bmatrix}
f_{s_{1}}(t) \\
0
\end{bmatrix} + \begin{bmatrix}
-f_{s_{2}}(t) \\
f_{s_{2}}(t)
\end{bmatrix} + \begin{bmatrix}
0 \\
f_{s_{3}}(t)
\end{bmatrix}\right) + \begin{bmatrix}
f_{e_{1}}(t) \\
f_{e_{2}}(t)
\end{bmatrix}
$$
If we pull out the scalars, we see:
$$
= - \left( f_{s_{1}}(t)\begin{bmatrix}
1 \\
0
\end{bmatrix}+f_{s_{2}}(t)\begin{bmatrix}
-1 \\
1
\end{bmatrix} +f_{s_{3}}(t)\begin{bmatrix}
0 \\
1
\end{bmatrix} \right) + \begin{bmatrix}
f_{e_{1}}(t) \\
f_{e_{2}}(t)
\end{bmatrix}
$$
Using our [[Linear Algebra/10 Matrix-Vector Multiplication/10.1 Matrix-Column-Vector Multiplication via Linear Combinations\|10.1 Matrix-Column-Vector Multiplication via Linear Combinations]] definition, we see
$$
\begin{align*}
&=  -\begin{bmatrix}
1 & -1 & 0 \\
0 & 1 & -1
\end{bmatrix}_{2 \times 3} \begin{bmatrix}
f_{s_{1}}(t) \\
f_{s_{2}}(t) \\
f_{s_{3}}(t)
\end{bmatrix}_{3 \times 1} + \begin{bmatrix}
f_{e_{1}}(t) \\
f_{e_{2}}(t)
\end{bmatrix}\\
&= -A^{T} \cdot \vec{f}_{s}(t) + \vec{f}_{e}(t)
\end{align*}
$$
Notice how our matrix is the transpose of our modeling matrix for the net spring force.

`\end{proof}`

---

> [!exercise] Matrix-Matrix Multiplication and Mass-Spring Chains
> How can we use [[Linear Algebra/11 Matrix-Matrix Multiplication/11 Matrix-Matrix Multiplication\|11 Matrix-Matrix Multiplication]] to represent our mass-spring chain system?

`\begin{proof}[Solution.]`
Let $-\vec{y}(t) = A^{T}\vec{f}_{s}(t)$.
$$
-A^{T} \cdot \vec{f}_{s}(t) + \vec{f}_{e}(t) = y(t)+\vec{f}_{e}(t)
$$
Recall net forces on masses:
$$
\begin{align*}
\begin{bmatrix}
\sum F_{1}(t) \\
\sum F_{2}(t)
\end{bmatrix} = \left[ \sum \vec{F}(t) \right]_{2 \times 1} &= \vec{y}(t) + \vec{f}_{e}(t)\\
&= -A^{T} \cdot \vec{f}_{s}(t)+\vec{f}_{e}(t)\\
&= -A^{T} \cdot C \cdot \vec{e}(t)+\vec{f}_{e}(t)\\
&= \underbrace{ [-A^{T}]_{2 \times 3} \cdot [C]_{3 \times 3} \cdot [A]_{3 \times 2}  }_{ \underset{ \text{stiffness matrix} }{ K_{2 \times 2}  }} \cdot [\vec{u}(t)]_{2 \times 1} + [\vec{f}e(t)]_{2 \times 1}\\
\implies \left[ \sum \vec{F}(t) \right]_{2 \times 1} &= -K \cdot \vec{u}(t) + \vec{f}_{e}(t)\\
\implies \begin{bmatrix}
\sum F_{1}(t) \\
\sum F_{2}(t)
\end{bmatrix} &= \begin{bmatrix}
m_{1} \cdot \ddot{u_{1}}(t) \\
m_{2} \cdot \ddot{u_{2}}(t)
\end{bmatrix}
\end{align*}
$$
Can this be a linear combination?
$$
\begin{align*}
&= \begin{bmatrix}
m_{1} \cdot  \ddot{u_{1}} +0\\
0+m_{2} \cdot  \ddot{u_{2}}
\end{bmatrix}\\
\begin{bmatrix}
\sum F_{1}(t) \\
\sum F_{2}(t)
\end{bmatrix} &= \begin{bmatrix}
m_{1} \cdot  \ddot{u_{1}} \\
0
\end{bmatrix}+\begin{bmatrix}
0\\
m_{2} \cdot  \ddot{u_{2}} 
\end{bmatrix}\\
&= \ddot{u_{1}}(t) \begin{bmatrix}
m_{1} \\
0
\end{bmatrix}+\ddot{u_{2}}\begin{bmatrix}
0 \\
m_{2}
\end{bmatrix}\\
&= \underbrace{ \begin{bmatrix}
m_{1} & 0 \\
0 & m_{2}
\end{bmatrix}_{2 \times 2} }_{ M_{2 \times 2} } \underbrace{ \begin{bmatrix}
\ddot{u_{1}}(t) \\
\ddot{u_{2}}(t)
\end{bmatrix}_{2 \times 1} }_{ [\ddot{\vec{u}}(t)]_{2 \times 1} }\\
\implies M\ddot{\vec{u}}(t) &= -K\vec{u}(t)+\vec{f}_{e}(t)\\
\implies M \cdot \ddot{\vec{u}}(t) + K\vec{u}(t) &= \vec{f}_{e}(t)
\end{align*}
$$

If we think back to when gravity is turned on,

$$
\ddot{\vec{u}}(t)=\begin{bmatrix}
0 \\
0
\end{bmatrix} \text{ since masses are at rest and } \vec{f}_{e}(t)= \begin{bmatrix}
9.8 \cdot m_{1} \\
9.8 \cdot m_{2}
\end{bmatrix}
$$

Therefore, we can represent our system as

$$
\begin{align*}
\implies M \cdot \cancelto{ \vec{0} }{ \ddot{\vec{u}}(t) } + K \vec{u}(t) &=  \vec{f}_{e}(t)\\
\implies K \vec{u}(t) &= \vec{f}_{e}(t)\\
\implies K \cdot \vec{u} &= \vec{f}_{e}
\end{align*}
$$

 `\end{proof}`