---
{"dg-publish":true,"permalink":"/linear-algebra/12-nonsingular-linear-systems/12-2-backwards-substitution/","tags":["Type/Theorem","Topic/Linear_Algebra"]}
---

Types: *N/A*
Examples: [[Linear Algebra/12 Nonsingular Linear Systems/12.2.1 Nonsingular Matrix to Model Gravity\|12.2.1 Nonsingular Matrix to Model Gravity]]
Constructions: *N/A*
Generalizations: *N/A*

Properties: *N/A*
Sufficiencies: *N/A*
Questions: *N/A*

> [!theorem|*] Backwards Substitution: Upper-Triangular $U\vec{x}=\vec{y}$
> 
> Let $U\vec{x} = \vec{y}$ be a given [[Linear Algebra/12 Nonsingular Linear Systems/12.1 The Square Linear-Systems Problem\|linear-systems problem]] with [[Linear Algebra/08 Anatomy of Matrices/8.9 Upper-Triangular Matrix\|8.9 Upper-Triangular Matrix]] $U \in \mathbb{R}^{n \times n}$ and $\vec{y} \in \mathbb{R}^{n}$. If entries of $U$, $u_{ii} \neq 0$ for all $i \in \{ 1,2,\dots,n \}$, then our linear-system problem has a unique solution. This solution can be found using the **backward substitution** algorithm:
> $$
> \begin{align*}
> x_{n} &= \frac{y_{n}}{u_{nn}}\\
> x_{i} &= \frac{1}{u_{ii}} \left( y_{i} - \sum_{j=i+1}^{n} u_{ij}x_{j} \right) 
> \end{align*}
> $$
> where $i = (n-1),(n-2), \dots, 2, 1$.

`\begin{proof}`
Let $n=5$ and consider
$$
\begin{bmatrix}
u_{11} & u_{12} & u_{13} & u_{14} & u_{15} \\
0 & u_{22} & u_{23} & u_{24} & u_{25} \\
0 & 0 & u_{33} & u_{34} & u_{35} \\
0 & 0 & 0 & u_{44} & u_{45} \\
0 & 0 & 0 & 0 & u_{55}
\end{bmatrix} \begin{bmatrix}
x_{1} \\
x_{2} \\
x_{3} \\
x_{4} \\
x_{5}
\end{bmatrix} = \begin{bmatrix}
y_{1} \\
y_{2} \\
y_{3} \\
y_{4} \\
y_{5}
\end{bmatrix}
$$
Note that $u_{ii} \neq 0$ for all $i \in [5)$.

# Step 0
Let's start at the bottom entry of the matrix.
$$
\begin{align*}
\text{Entry}_{5}(U \vec{x}) &= y_{5}\\
\implies [\text{Row}_{5}(U)]_{1 \times 5} [\vec{x}]_{5 \times 1} &= y_{5}\\
&= \begin{bmatrix}
0 & 0 & 0 & 0 & u_{55}
\end{bmatrix}\begin{bmatrix}
x_{1} \\
x_{2} \\
x_{3} \\
x_{4} \\
x_{5}
\end{bmatrix}\\
\implies u_{55} \cdot x_{5} &= y_{5}\\
\implies x_{5} &= \frac{y_{5}}{u_{55}}
\end{align*}
$$
From this, we can work "backwards" up the matrix. In our next step, we will substitute in our value we get for $x_{5}$.

# Step 1
Because we solved for a value of $x_{5}$ in our last step, we can substitute it in when solving for $x_{4}$.
$$
\begin{align*}
\implies \text{Entry}_{4} (U \cdot \vec{x}) &= y_{4}\\
\implies \text{Row}_{4}(U) \cdot \vec{x} &= y_{4}\\
\implies \begin{bmatrix}
0 & 0 & 0 & u_{44} & u_{45}
\end{bmatrix} \begin{bmatrix}
x_{1} \\
x_{2} \\
x_{3} \\
x_{4} \\
\boxed{x_{5}}
\end{bmatrix} &= y_{4}\\
\implies u_{44} \cdot x_{4} + u_{45} \cdot x_{5} &= y_{4}\\
\implies u_{44} \cdot x_{4} &= y_{4}-u_{45}x_{5}\\
\implies x_{4} &= \frac{1}{u_{44}}(y_{4}-u_{45}x_{5})
\end{align*} 
$$
# Step 2
We continue our algorithm by solving for $x_{3}$.
$$
\begin{align*}
\implies \text{Entry}_{3}(U \cdot \vec{x}) &= y_{3}\\
\implies \text{Row}_{3}(U) \cdot \vec{x} &= y_{3}\\
\implies \begin{bmatrix}
0 & 0 & u_{33} & u_{34} & u_{35}
\end{bmatrix} \begin{bmatrix}
x_{1} \\
x_{2} \\
x_{3} \\
\boxed{x_{4}} \\
\boxed{x_{5}}
\end{bmatrix}&= y_{3}\\
\implies u_{33}x_{3} + u_{34}x_{4} + u_{35}x_{5} &= y_{3}\\
\implies x_{3} &= \frac{1}{u_{33}} \left( y_{3} -u_{34}x_{4} - u_{35}x_{5}\right) 
\end{align*}
$$
Can we generalize this?
$$
\implies x_{3} = \frac{1}{u_{33}} \left( y_{3} - \sum_{k=4}^{5} u_{3k} \cdot x_{k} \right) 
$$
Let's look back at $x_{4}$ from Step 1. Can we generalize that too?
$$
\begin{align*}
x_{4} &= \frac{1}{u_{44}}(y_{4}-u_{45}x_{5})\\
&= \frac{1}{u_{44}} \left( y_{4} - \sum_{k=5}^{5}u_{4k} \cdot x_{k} \right) 
\end{align*}
$$

# Step 3
Can we intuit what our final entries will look like based on the pattern we've been seeing? Let's find $x_{2}$ first.
$$
\begin{align*}
\text{Entry}_{2} (U \cdot \vec{x}) &= y_{2}\\
x_{2} &= \frac{1}{u_{22}} \left( y_{2} - \sum_{k=3}^{5} u_{2k} \cdot x_{k} \right)\\
&\iff \text{Row}_{2} (U) \cdot \vec{x}=y_{2}\\
&\implies \begin{bmatrix}
0 & u_{22} & u_{23} & u_{24} & u_{25}
\end{bmatrix}\begin{bmatrix}
x_{1} \\
x_{2} \\
\boxed{x_{3}} \\
\boxed{x_{4}} \\
\boxed{x_{5}}
\end{bmatrix}=y_{2}\\
&\implies u_{22}x_{2}+u_{23}x_{3}+u_{24}x_{4}+u_{25}x_{5} =y_{2}\\
&\implies x_{2} = \frac{1}{u_{22}} \left( y_{2}-u_{23}x_{3}-u_{24}x_{4}-u_{25}x_{5} \right) 
\end{align*}
$$
Therefore, to get our final entry,
$$
\begin{align*}
x_{1} &= \frac{1}{u_{11}}\left( y_{1} - \sum_{k=2}^{5}u_{1k}x_{k} \right) 
\end{align*}
$$
`\end{proof}`