---
{"dg-publish":true,"permalink":"/linear-algebra/12-nonsingular-linear-systems/12-5-forward-substitution/","tags":["Topic/Linear_Algebra","Type/Theorem"]}
---

Types: *N/A*
Examples: *N/A*
Constructions: *N/A*
Generalizations: *N/A*

Properties: *N/A*
Sufficiencies: *N/A*
Questions: *N/A*

> [!theorem|*] Forward Substitution: Lower-Triangular $L\vec{x}=\vec{b}$
> 
> Let $L \vec{x} = \vec{b}$ be a given [[Linear Algebra/12 Nonsingular Linear Systems/12.1 The Square Linear-Systems Problem\|12.1 The Square Linear-Systems Problem]] problem with [[Linear Algebra/08 Anatomy of Matrices/8.7 Lower-Triangular Matrix\|8.7 Lower-Triangular Matrix]] $L \in \mathbb{R}^{n \times n}$ and $\vec{b} \in \mathbb{R}^{n}$. If diagonal values $u_{ii} \neq 0$ for all $i \in \{ 1,2,\dots,n \}$, then our linear-system problem has a unique solution. This solution can be found using the **forward substitution** algorithm:
> $$
> \begin{align*}
> x_{1} &= \frac{b_{1}}{u_{11}}\\
> x_{i} &= \frac{1}{u_{ii}} \left( b_{i} - \sum_{j=1}^{i-1} u_{ij}x_{j} \right) 
> \end{align*}
> $$
> where $i = 2,3,\dots,n$.

**Remark.** In addition to solving problems involving [[Linear Algebra/08 Anatomy of Matrices/8.9 Upper-Triangular Matrix\|8.9 Upper-Triangular Matrix]], we also use [[Linear Algebra/08 Anatomy of Matrices/8.7 Lower-Triangular Matrix\|8.7 Lower-Triangular Matrix]] for the [[Linear Algebra/12 Nonsingular Linear Systems/12.1 The Square Linear-Systems Problem\|12.1 The Square Linear-Systems Problem]].
$$
L \cdot \textcolor{red}{\vec{y}} = \vec{b}
$$
 <span style='float:right;'>$\blacklozenge$</span>
`\begin{proof}[Informal Proof.]`
Let's look at a system of 4 linear equations in 4 unknowns with a lower-triangular coefficient matrix $L$. Suppose
$$
\begin{align*}
\begin{bmatrix}
l_{11} & 0 & 0 & 0 \\
l_{21} & l_{22} & 0 & 0 \\
l_{31} & l_{32} & l_{33} & 0 \\
l_{41} & l_{42} & l_{43} & l_{44}
\end{bmatrix} \begin{bmatrix}
\textcolor{red}{y_{1}} \\
\textcolor{red}{y_{2}} \\ 
\textcolor{red}{y_{3}} \\
\textcolor{red}{y_{4}}
\end{bmatrix} &= \begin{bmatrix}
b_{1} \\
b_{2} \\
b_{3} \\
b_{4}
\end{bmatrix}
\end{align*}
$$
Let's look at the individual row entries of the left and right hand side.
$$
\begin{align*}
&l_{11}\textcolor{red}{y_{1}} &+0 &+0 &+0 &= b_{1}\\
&l_{21} \textcolor{red}{y_{1}}&+l_{22}\textcolor{red}{y_{2}} &+ 0 &+ 0 &= b_{2}\\
&l_{31} \textcolor{red}{y_{1}} &+ l_{32} \textcolor{red}{y_{2}} &+ l_{33} \textcolor{red}{y_{3}} &+ 0 &= b_{3}\\
&l_{41} \textcolor{red}{y_{1}} &+ l_{42} \textcolor{red}{y_{2}} &+ l_{43} \textcolor{red}{y_{3}} &+ l_{44} \textcolor{red}{y_{4}} &= b_{4}
\end{align*}
$$
Notice that the first equation has only one unknown. Furthermore, if $u_{ii} \neq 0$ for all $i$, we solve for the unknown
$$
\textcolor{red}{y_{1}} = \frac{1}{l_{11}} \cdot (b_{1})
$$
Because we know $y_{1}$, we can continue and solve for $y_{2}$ and so on.
$$
l_{21}y_{1} + l_{22}\textcolor{red}{y_{2}}=b_{2} \implies \textcolor{red}{y_{2}} = \frac{1}{l_{22}} \cdot (b_{4} - l_{21}y_{1})
$$
We continue with row 3 for $y_{3}$.
$$
\begin{align*}
l_{31}y_{1} + l_{32}y_{2} + l_{33} \textcolor{red}{y_{3}} = b_{3} &\implies \textcolor{red}{y_{3}} = \frac{1}{l_{33}} (b_{3} - l_{31}y_{1} - l_{32}y_{2} )\\
&\implies \textcolor{red}{y_{3}} =\frac{1}{l_{33}}\left( b_{3}-\sum_{j=1}^{2}l_{3j}y_{j} \right) 
\end{align*}
$$
Finally, we can find $y_{4}$.
$$
\begin{align}
l_{41}y_{1}+l_{42}y_{2}+l_{43}y_{3} +l_{44}\textcolor{red}{y_{4}}  & \implies \textcolor{red}{y_{4}} = \frac{1}{l_{44}} (b_{4} - l_{41}y_{1}-l_{42}y_{2}-l_{43}y_{3}) \\
 & \implies \textcolor{red}{y_{4}} = \frac{1}{l_{44}} \left( b_{4} - \sum_{j=1}^{3}u_{4j}y_{j} \right) 
\end{align}
$$
We have now solved our linear systems problem for unknowns $y_{i}$ using forward substitution.
`\end{proof}`