---
{"dg-publish":true,"permalink":"/linear-algebra/05-inner-products-and-vector-norms/5-6-law-of-cosines/","tags":["Type/Theorem","Topic/Trigonometry"]}
---

Types: *N/A*
Examples: *N/A*
Constructions: [[Linear Algebra/05 Inner Products and Vector Norms/5.7 Cosine Formula for Inner Product\|5.7 Cosine Formula for Inner Product]]
Generalizations: *N/A*

Properties: *N/A*
Sufficiencies: [[Linear Algebra/05 Inner Products and Vector Norms/5.5 Pythagorean Theorem\|5.5 Pythagorean Theorem]]
Questions: *N/A*

> [!theorem|*] Law of Cosines
> Let $a, b, c$ be positive real numbers representing the length of the three sides of any triangle. Let $\theta$ be the angle opposite the side length of $c$ and between the sides of lengths $a$ and $b$. Then,
> $$c^{2} = a^{2} + b^{2} - 2ab\cos(\theta)$$

`\begin{proof}`Let's break the theorem statement into two cases:
1. The Acute Case $\left( 0 < \theta < \frac{\pi}{2} \right)$
   
<div class="transclusion internal-embed is-loaded"><div class="markdown-embed">




==⚠  Switch to EXCALIDRAW VIEW in the MORE OPTIONS menu of this document. ⚠==


# Text Elements
# Embedded files
9dc03aef1bd9be767817c5d11f87ea50ba1ebf2d: $\theta$
c698f5c42cefbd2ac7b5c8969549ee89068b5bfb: $b$
5819e66fe6437fb7757e7b6f3a7463b0c0f1ddd7: $x$
7f48413a83c3587e255b2ad1eaf331ce65187901: $a-x$
33c1ac43d1fce37257312ff93de2bcce95e366c3: $c$
70ee5b828338e6639bda4ef94af6041c620e91f5: $h$
7a2958810c301cd73bd698adad7ea9af703d578c: $\theta$
0a1fb8e43a34c50c96da6b3cbd419fca1f05ac00: $b$
43c0d15551f72b91e67f3ac64a8e61dd762b7fbe: $x$
4b5749a4ad00913a3436bcac4a6b68225d531b1c: $a-x$
605e2242cde1e023beb6525ee5db9ebd32a4330f: $h$
648399c5d1d86dca1e07f315edc46826689375c9: $c$



</div></div>

   In this case, we have $x^{2} + h^{2} = b^{2}$. Further, we see:
   $$
\begin{align*}
c^{2} &= (a-x)^{2}+h^{2}\\
&= a^{2}-2ax+x^{2}+h^{2}\\
&= a^{2}-2ax+b^{2}
\end{align*}
$$
Take a look at the right triangle on the left. 
$$
\begin{align*}
\cos \theta&= \frac{x}{b}\\
\implies b\cos \theta&= x
\end{align*}
$$
If we sub in $b\cos \theta$  for $x$ into our formula for $c^{2}$, we get
$$
a^{2}+b^{2}-2ab\cos \theta
$$
   which is what we wanted to show.
1. The Obtuse Case $\left( \frac{\pi}{2} < \theta < \pi \right)$
   
<div class="transclusion internal-embed is-loaded"><div class="markdown-embed">

<div class="markdown-embed-title">

# 500

</div>



==⚠  Switch to EXCALIDRAW VIEW in the MORE OPTIONS menu of this document. ⚠==


# Text Elements
# Embedded files
9dc03aef1bd9be767817c5d11f87ea50ba1ebf2d: $\theta$
c698f5c42cefbd2ac7b5c8969549ee89068b5bfb: $b$
5819e66fe6437fb7757e7b6f3a7463b0c0f1ddd7: $x$
7f48413a83c3587e255b2ad1eaf331ce65187901: $a-x$
33c1ac43d1fce37257312ff93de2bcce95e366c3: $c$
70ee5b828338e6639bda4ef94af6041c620e91f5: $h$
7a2958810c301cd73bd698adad7ea9af703d578c: $\theta$
0a1fb8e43a34c50c96da6b3cbd419fca1f05ac00: $b$
43c0d15551f72b91e67f3ac64a8e61dd762b7fbe: $x$
4b5749a4ad00913a3436bcac4a6b68225d531b1c: $a-x$
605e2242cde1e023beb6525ee5db9ebd32a4330f: $h$
648399c5d1d86dca1e07f315edc46826689375c9: $c$



</div></div>

   Again, we have $x^{2} + h^{2} = b^{2}$ on the left triangle. On the triangle to the right of $h$, we see:
   $$
\begin{align*}
c^{2} &= (a-x)^{2}+h^{2}\\
&= a^{2}-2ax+x^{2}+h^{2}\\
&= a^{2} - 2ax + b^{2}
\end{align*}
$$
Let's look at the triangle on the left again.
$$
\begin{align*}
\cos \theta &= \frac{x}{b}\\
\implies b \cos \theta &= x
\end{align*}
$$
Therefore,
$$
\begin{align*}
c^{2} &= a^{2} - 2ab\cos \theta + b^{2}\\
&= a^{2} + b^{2} - 2ab\cos \theta
\end{align*}
$$
   
`\end{proof}`